Common.v
@@ -1,0 +1,10 @@
+
+From Coq Require Import ZArith Lia Bool List String Program.Equality.
+Local Open Scope Z_scope.
+
+Local Open Scope string_scope.
+  Definition ident := string.
+  Definition store : Type := ident -> Z.
+  Definition sempty : store := (fun _ => 0).
+  Definition supdate (x: ident) (v: Z) (s: store) : store :=
+    fun y => if string_dec x y then v else s y.
